Fix noncompiling bits from previous commit

src/Parsers/ParserFromParserADT.v
@@ -1,19 +1,19 @@
 (** Reference implementation of a splitter and parser based on that splitter *)
 Require Import Coq.Strings.String.
-Require Import Fiat.Parsers.SplitterFromParserADT.
-Require Import Fiat.Parsers.ContextFreeGrammar.Notations.
-Require Export Fiat.Parsers.ParserImplementationOptimized.
+Require Import Fiat.Common.BoundedLookup.
 Require Import Fiat.ADT.ComputationalADT.
 Require Import Fiat.ADTRefinement.GeneralRefinements.
+Require Import Fiat.ADTRefinement.Core.
+Require Import Fiat.ADTNotation.BuildADTSig.
+Require Import Fiat.Parsers.ContextFreeGrammar.Notations.
 Require Import Fiat.Parsers.ParserADTSpecification.
 Require Import Fiat.Parsers.ContextFreeGrammar.Valid.
 Require Import Fiat.Parsers.ContextFreeGrammar.ValidReflective.
 Require Import Fiat.Parsers.ContextFreeGrammar.Transfer.
+Require Export Fiat.Parsers.ParserImplementationOptimized.
+Require Import Fiat.Parsers.SplitterFromParserADT.
 Require Import Fiat.Parsers.BooleanRecognizerEquality.
 Require Import Fiat.Parsers.BaseTypes.
-Require Import Fiat.ADTRefinement.Core.
-Require Import Fiat.Common.BoundedLookup.
-Require Import Fiat.ADTNotation.BuildADTSig.
 Require Import Fiat.Parsers.StringLike.Core.
 
 Set Implicit Arguments.
@@ -34,7 +34,7 @@ Section parser.
 
   Definition newS := ibound (indexb (@Build_BoundedIndex _ _ (ConstructorNames (string_rep Ascii.ascii String.string Carriers.default_production_carrierT)) "new" _ )).
 
-  Definition new_string_of_base_string (str : @String _ stringlike_stringlike)
+  Definition new_string_of_base_string (str : @String _ stringlike_stringlikemin)
     := (cConstructors (projT1 splitter_impl) newS str).
 
   Lemma new_string_of_base_string_R {str}
@@ -56,14 +56,14 @@ Section parser.
              str
              new_string_of_base_string_R)).
 
-  Local Instance split_dataProj : @split_dataT _ (adt_based_StringLike_lite splitter_impl) (RDPList.rdp_list_predata (G := G))
+  Local Instance split_dataProj : @split_dataT _ (adt_based_StringLikeMin_lite splitter_impl) (RDPList.rdp_list_predata (G := G))
     := { split_string_for_production idx str offset len := msplits splitter_impl idx offset len str }.
 
   Local Instance adtProj
   : @StringLikeProj
       _
       (adt_based_splitter splitter_impl)
-      (adt_based_StringLike_lite splitter_impl)
+      (adt_based_StringLikeMin_lite splitter_impl)
       (ParserImplementation.parser_data (adt_based_splitter splitter_impl))
       split_dataProj
     := { proj := @proj1_sig _ _ }.
@@ -76,8 +76,7 @@ Section parser.
   Definition parser' : Parser G stringlike_stringlike.
   Proof.
     refine (@parser ls Hvalid (adt_based_splitter splitter_impl)
-                    (adt_based_StringLike_lite splitter_impl)
-                    _
+                    (adt_based_StringLikeMin_lite splitter_impl)
                     _
                     adtProj
                     stringlike_stringlikemin
@@ -186,7 +185,7 @@ Definition parser
 Proof.
   let term := (eval cbv beta delta [parser''] in (@parser'' HSLM HSL HSLP ls Hvalid splitter_impl)) in
   refine (term _ _).
-  cbv beta iota zeta delta [has_parse parser' parser transfer_parser new_string_of_string proj adtProj proj1_sig new_string_of_base_string cConstructors StringLike.length adt_based_StringLikeMin adt_based_StringLikeMin_lite adt_based_StringLike_lite pdata data' BaseTypes.split_string_for_production split_dataProj adt_based_splitter BuildComputationalADT.callcADTMethod ibound indexb cMethods cRep BaseTypes.predata ParserImplementation.parser_data StringLikeMin_of_StringLike adt_based_StringLike RDPList.rdp_list_predata RDPList.rdp_list_nonterminals_listT list_to_grammar Valid_nonterminals RDPList.rdp_list_is_valid_nonterminal RDPList.rdp_list_remove_nonterminal list_to_productions newS Fin.R mto_string msplits drop take is_char String length get bool_eq beq mlength mchar_at_matches mdrop mtake mget].
+  cbv beta iota zeta delta [has_parse parser' parser transfer_parser new_string_of_string proj adtProj proj1_sig new_string_of_base_string cConstructors StringLike.length adt_based_StringLikeMin adt_based_StringLikeMin_lite adt_based_StringLike_lite pdata data' BaseTypes.split_string_for_production split_dataProj adt_based_splitter BuildComputationalADT.callcADTMethod ibound indexb cMethods cRep BaseTypes.predata ParserImplementation.parser_data adt_based_StringLike RDPList.rdp_list_predata RDPList.rdp_list_nonterminals_listT list_to_grammar Valid_nonterminals RDPList.rdp_list_is_valid_nonterminal RDPList.rdp_list_remove_nonterminal list_to_productions newS Fin.R mto_string msplits drop take is_char String length get bool_eq beq mlength mchar_at_matches mdrop mtake mget].
   change_opt ls nt str.
   match goal with
     | [ |- _ = ?x :> ?T ] => instantiate (1 := x); exact_no_check (@eq_refl T x)
